src/computational_monads/simulation_semantics/constructions/uniform_oracle.lean
@@ -5,7 +5,6 @@ open oracle_comp oracle_spec
 
 variables {A B : Type} {spec spec' spec'' : oracle_spec}
 
-@[simps]
 noncomputable def uniform_oracle (spec : oracle_spec) [spec.finite_range] : 
   simulation_oracle spec uniform_selecting :=
 ⟪λ i t, $ᵗ (spec.range i)⟫
@@ -19,11 +18,11 @@ noncomputable instance S_unique : unique (uniform_oracle spec).S := stateless_or
 
 @[simp]
 lemma apply_eq (i : spec.ι) (t : spec.domain i) (u : unit) :
-  (uniform_oracle spec).o i (t, u) = $ᵗ (spec.range i) >>= λ u, return (u, ()) := rfl
+  (uniform_oracle spec) i (t, u) = $ᵗ (spec.range i) >>= λ u, return (u, ()) := rfl
 
 @[simp]
 lemma support_apply (i : spec.ι) (t : spec.domain i) (u : unit) :
-  ((uniform_oracle spec).o i (t, u)).support = ⊤ :=
+  ((uniform_oracle spec) i (t, u)).support = ⊤ :=
 by simp only [set.eq_univ_iff_forall, apply_eq, support_bind, support_uniform_select_fintype,
   set.top_eq_univ, support_pure, set.Union_true, set.Union_singleton_eq_range, set.mem_range,
   prod.forall, prod.mk.inj_iff, exists_eq_left, forall_const, eq_iff_true_of_subsingleton]
