src/computational_monads/simulation_semantics/default_simulate.lean
@@ -9,6 +9,7 @@ variables {α β γ : Type} {spec spec' spec'' : oracle_spec}
 
 section default_simulate
 
+-- TODO: should this go farther and be `notation` instead of `inline`?
 @[inline, reducible]
 def default_simulate (so : simulation_oracle spec spec') (oa : oracle_comp spec α) :
   oracle_comp spec' (α × so.S) := oa.simulate so so.default_state
@@ -26,7 +27,7 @@ lemma default_simulate_bind' : default_simulate so (bind' α β oa ob) =
   simulate so oa so.default_state >>= λ x, simulate so (ob x.1) x.2 := rfl
 
 lemma default_simulate_query : default_simulate so (query i t) =
-  so.o i (t, so.default_state) := rfl
+  so i (t, so.default_state) := rfl
 
 lemma default_simulate_map : default_simulate so (f <$> oa) =
   simulate so oa so.default_state >>= return ∘ prod.map f id := rfl
@@ -55,7 +56,7 @@ lemma support_default_simulate_bind' : (default_simulate so (bind' α β oa ob))
   ⋃ x ∈ (default_simulate so oa).support, (simulate so (ob $ prod.fst x) x.2).support := rfl
 
 lemma support_default_simulate_query : (default_simulate so (query i t)).support =
-  (so.o i (t, so.default_state)).support := rfl
+  (so i (t, so.default_state)).support := rfl
 
 lemma support_default_simulate_map : (default_simulate so (f <$> oa)).support =
   prod.map f id '' (default_simulate _ oa).support := support_simulate_map so oa _ f
@@ -100,7 +101,7 @@ lemma eval_dist_default_simulate_bind' : ⦃default_simulate so (bind' α β oa 
 eval_dist_simulate_bind so oa ob so.default_state
 
 lemma eval_dist_default_simulate_query :
-  ⦃default_simulate so (query i t)⦄ = ⦃so.o i (t, so.default_state)⦄ :=
+  ⦃default_simulate so (query i t)⦄ = ⦃so i (t, so.default_state)⦄ :=
 eval_dist_simulate_query so i t so.default_state
 
 lemma eval_dist_default_simulate_map :
@@ -130,7 +131,7 @@ lemma default_simulate_bind'_equiv : default_simulate so (bind' α β oa ob) ≃
   default_simulate so oa >>= λ x, simulate so (ob x.1) x.2 := rfl
 
 lemma default_simulate_query_equiv : default_simulate so (query i t) ≃ₚ
-  so.o i (t, so.default_state) := rfl
+  so i (t, so.default_state) := rfl
 
 lemma default_simulate_map_equiv : default_simulate so (f <$> oa) ≃ₚ
   prod.map f id <$> simulate so oa so.default_state := simulate_map_equiv so oa _ f
@@ -163,7 +164,7 @@ lemma default_simulate'_bind' : default_simulate' so (bind' α β oa ob) =
   prod.fst <$> (default_simulate so oa >>= λ x, simulate so (ob x.1) x.2) := rfl
 
 lemma default_simulate'_query : default_simulate' so (query i t) =
-  prod.fst <$>so.o i (t, so.default_state) := rfl
+  prod.fst <$>so i (t, so.default_state) := rfl
 
 section support
 
@@ -185,7 +186,7 @@ lemma support_default_simulate'_bind : (default_simulate' so (oa >>= ob)).suppor
 by simp [set.image_Union]
 
 lemma support_default_simulate'_query : (default_simulate' so (query i t)).support =
-  prod.fst '' (so.o i (t, so.default_state)).support := support_simulate'_query so i t _
+  prod.fst '' (so i (t, so.default_state)).support := support_simulate'_query so i t _
 
 lemma support_default_simulate'_map : (default_simulate' so (f <$> oa)).support =
   f '' (simulate' so oa so.default_state).support :=
@@ -202,7 +203,7 @@ mem_support_of_mem_support_simulate' so oa so.default_state hx
 then the first value of simulation has the same support as the original computation.
 For example simulation with the identity oracle `idₛ` doesn't change the support -/
 theorem support_default_simulate'_eq_support [subsingleton so.S]
-  (h : ∀ i t, prod.fst '' (so.o i (t, so.default_state)).support = ⊤) :
+  (h : ∀ i t, prod.fst '' (so i (t, so.default_state)).support = ⊤) :
   (default_simulate' so oa).support = oa.support :=
 support_simulate'_eq_support so oa so.default_state
   (λ i t s, subsingleton.elim so.default_state s ▸ h i t)
@@ -238,7 +239,7 @@ lemma eval_dist_default_simulate'_bind' : ⦃default_simulate' so (bind' α β o
 eval_dist_simulate'_bind so oa ob so.default_state
 
 lemma eval_dist_default_simulate'_query : ⦃default_simulate' so (query i t)⦄ =
-  ⦃so.o i (t, so.default_state)⦄.map prod.fst :=
+  ⦃so i (t, so.default_state)⦄.map prod.fst :=
 eval_dist_simulate'_query so i t so.default_state
 
 lemma eval_dist_default_simulate'_map : ⦃default_simulate' so (f <$> oa)⦄ =
@@ -271,7 +272,7 @@ lemma default_simulate'_bind'_equiv : default_simulate' so (bind' α β oa ob) �
 simulate'_bind_equiv so oa ob so.default_state
 
 lemma default_simulate'_query_equiv : default_simulate' so (query i t) ≃ₚ
-  prod.fst <$> (so.o i (t, so.default_state)) := simulate'_query_equiv so i t so.default_state
+  prod.fst <$> (so i (t, so.default_state)) := simulate'_query_equiv so i t so.default_state
 
 @[simp]
 lemma default_simulate'_map_equiv : default_simulate' so (f <$> oa) ≃ₚ
